symbolic evaluation proofs for bytes and words.

src/ndep/SymEval.v
@@ -106,9 +106,6 @@ Section search_read_write.
 
       congruence.
     Qed.
-
-    
-
   End arg.
 
   Variable impures : FM.t (list (list (expr types))).
@@ -355,6 +352,165 @@ Module Evaluator (B : Heap) (ST : SepTheoryX.SepTheoryXType B).
         |}); 
       abstract (simpl; intros; congruence).
       Defined.
+
+      Variable sfuncs : list (ssignature btypes (tvType pcIndex) (tvType stateIndex)).
+
+      Variable known : list nat. 
+      Variable evals : hlist (fun n : nat => match nth_error sfuncs n with
+                                               | None => Empty_set 
+                                               | Some ss => SymEval_byte ss
+                                             end) known.
+
+      Definition symeval_read_byte (hyps : list (expr btypes)) (p : expr btypes) 
+        (s : SHeap btypes (tvType pcIndex) (tvType stateIndex))
+        : option (expr btypes) :=
+        let hyps := hyps ++ pures s in
+        let reader _ seb args := 
+          sym_read_byte seb hyps args p
+        in
+        fold_known _ _  reader (impures s) evals.
+
+      Theorem symeval_read_byte_correct : forall cs stn hyps funcs pe ve s uvars vars (m : B.mem),
+        symeval_read_byte hyps pe s = Some ve ->
+        AllProvable funcs uvars vars hyps ->
+        (exists sm, 
+          ST.satisfies cs (sexprD funcs sfuncs uvars vars (sheapD s)) stn sm
+          /\ ST.HT.satisfies sm m) ->
+        match exprD_ptr funcs uvars vars pe , exprD_byte funcs uvars vars ve with
+          | Some p , Some v => 
+            B.mem_get m p = Some v
+          | _ , _ => False
+        end.
+      Proof.
+        unfold symeval_read_byte. intros.
+        eapply fold_known_correct in H.
+        do 5 destruct H. destruct H1.
+        intuition.
+
+        generalize (sheapD_pures _ _ _ _ _ H); intros.
+
+        eapply sheapD_pull_impure 
+          with (funcs := funcs) (sfuncs := sfuncs) (a := uvars) (c := vars0) (cs := cs)
+            in H1.
+        apply In_split in H3. destruct H3. destruct H3.
+        subst. rewrite starred_In in H1.
+
+        eapply sym_read_byte_correct 
+          with (funcs := funcs) (uvars := uvars) (vars := vars0) (cs := cs) (stn := stn) (m := x4)
+            (P := sexprD funcs sfuncs uvars vars0 (Star
+          (sheapD
+            {|
+              impures := FM.remove x (impures s);
+              pures := pures s;
+              other := other s |})
+          (starred (Func x) (x5 ++ x6) Emp)))
+            in H6.
+        destruct (exprD_ptr funcs uvars vars0 pe); auto.
+        destruct (exprD_byte funcs uvars vars0 ve); auto.
+        erewrite ST.HT.satisfies_get; eauto.
+
+        eapply AllProvable_app; auto.
+
+        unfold heq in *.
+        rewrite H1 in H. simpl in *. rewrite ST.heq_star_comm in H.
+        rewrite H2 in *. rewrite ST.heq_star_assoc in H.
+        rewrite ST.heq_star_comm in H. rewrite ST.heq_star_assoc in H.
+        generalize H. clear.
+        match goal with 
+          | [ |- context [ applyD ?A ?B ?C ?D ?E ] ] =>
+            destruct (applyD A B C D E)
+        end; auto.
+        clear. intros.
+        eapply ST.satisfies_star in H. do 2 destruct H. intuition.
+        eapply ST.satisfies_pure in H0. PropXTac.propxFo.
+      Qed.
+
+      Definition symeval_write_byte (hyps : list (expr btypes)) (p v : expr btypes) 
+        (s : SHeap btypes (tvType pcIndex) (tvType stateIndex))
+        : option (SHeap btypes (tvType pcIndex) (tvType stateIndex)) :=
+        let hyps := hyps ++ pures s in
+        let writer _ seb args := 
+          sym_write_byte seb hyps args p v
+        in
+        match fold_known_update _ _ writer (impures s) evals with
+          | None => None
+          | Some i' => Some {| impures := i' ; pures := pures s ; other := other s |}
+        end.
+
+      Theorem symeval_write_byte_correct : forall cs stn hyps funcs pe ve v s s' uvars vars (m : B.mem),
+        symeval_write_byte hyps pe ve s = Some s' ->
+        AllProvable funcs uvars vars hyps ->
+        exprD_byte funcs uvars vars ve = Some v ->
+        (exists sm, 
+          ST.satisfies cs (sexprD funcs sfuncs uvars vars (sheapD s)) stn sm
+          /\ ST.HT.satisfies sm m) ->
+        match exprD_ptr funcs uvars vars pe with
+          | Some p =>
+            exists sm, 
+              ST.satisfies cs (sexprD funcs sfuncs uvars vars (sheapD s')) stn sm
+              /\ ST.HT.satisfies sm (B.mem_set m p v)
+          | _ => False
+        end.
+      Proof.
+        unfold symeval_write_byte. intros.
+        generalize dependent H.
+        match goal with
+          | [ |- context [ fold_known_update ?A ?B ?C ?D ?E ] ] =>
+            case_eq (fold_known_update A B C D E); intros; try congruence
+        end.
+        eapply fold_known_update_correct in H.
+        do 5 destruct H. destruct H2.
+        intuition. inversion H3; clear H3; subst. 
+        
+        eapply fold_args_update_correct in H6.
+        repeat match goal with
+                 | [ H : exists x, _ |- _ ] => destruct H
+               end. intuition; subst.
+        generalize (sheapD_pures _ _ _ _ _ H4).
+        rewrite sheapD_pull_impure in H4 by eauto.
+        rewrite starred_In in H4.
+        rewrite <- heq_star_assoc in H4. rewrite heq_star_comm in H4.
+        
+        simpl in *. rewrite H2 in *.
+        intros.
+
+        eapply sym_write_byte_correct 
+          with (P := ST.star
+            (sexprD funcs sfuncs uvars vars0
+              (sheapD
+                {|
+                  impures := FM.remove x (impures s);
+                  pures := pures s;
+                  other := other s |}))
+            (sexprD funcs sfuncs uvars vars0 (starred (Func x) (x5 ++ x6) Emp)))
+            (stn := stn) (cs := cs) (m := x4)
+          in H3; eauto.
+        2: apply AllProvable_app; eauto.
+        destruct (exprD_ptr funcs uvars vars0 pe); eauto.
+        unfold tvarD in H3.
+        exists (ST.HT.smem_set a v x4). split.
+        2: eapply ST.HT.satisfies_set; eauto.
+        rewrite sheapD_pull_impure.
+        2: eapply FM.find_add.
+        rewrite starred_In.
+        simpl. rewrite H2. generalize dependent H3. 
+        match goal with
+          | [ |- context [ applyD ?A ?B ?C ?D ?E ] ] =>
+            case_eq (applyD A B C D E)
+        end. intros.
+        rewrite <- ST.heq_star_assoc. rewrite ST.heq_star_comm. 
+        rewrite FM.remove_add. eapply H7.
+        intros; exfalso; auto.
+
+        unfold tvarD. generalize dependent H4.
+        match goal with
+          | [ |- context [ applyD ?A ?B ?C ?D ?E ] ] =>
+            case_eq (applyD A B C D E)
+        end. intros. auto.
+        intros. eapply ST.satisfies_star in H7.
+        do 2 destruct H7. intuition.
+        apply ST.satisfies_pure in H8. PropXTac.propxFo.
+      Qed.
     End ByteAccess.
 
     (** * Words *)
@@ -489,19 +645,19 @@ Module Evaluator (B : Heap) (ST : SepTheoryX.SepTheoryXType B).
         eapply sheapD_pull_impure 
           with (funcs := funcs) (sfuncs := sfuncs) (a := uvars) (c := vars0) (cs := cs)
             in H1.
-        eapply starred_In in H3.
-        destruct H3. rewrite H3 in H1.
+        destruct (In_split _ _ H3). destruct H7. subst.
+        rewrite starred_In in H1.
 
         eapply sym_read_word_correct 
           with (funcs := funcs) (uvars := uvars) (vars := vars0) (cs := cs) (stn := stn) (m := x4)
-            in H6.
-        3: instantiate (1 := sexprD funcs sfuncs uvars vars0 (Star
+            (P := sexprD funcs sfuncs uvars vars0 (Star
           (sheapD
             {|
               impures := FM.remove x (impures s);
               pures := pures s;
               other := other s |})
-          (starred (Func x) x5 Emp))).
+          (starred (Func x) (x5 ++ x6) Emp)))
+            in H6.
         destruct (exprD_ptr_w funcs uvars vars0 pe); auto.
         destruct (exprD_word funcs uvars vars0 ve); auto.
         erewrite ST.HT.satisfies_get_word; eauto.
@@ -534,18 +690,19 @@ Module Evaluator (B : Heap) (ST : SepTheoryX.SepTheoryXType B).
           | Some i' => Some {| impures := i' ; pures := pures s ; other := other s |}
         end.
 
-      Theorem symeval_write_word_correct : forall cs stn hyps funcs pe ve s s' uvars vars m,
+      Theorem symeval_write_word_correct : forall cs stn hyps funcs pe ve s s' uvars vars m v,
         symeval_write_word hyps pe ve s = Some s' ->
         AllProvable funcs uvars vars hyps ->
+        exprD_word funcs uvars vars ve = Some v ->
         (exists sm, 
              ST.satisfies cs (sexprD funcs sfuncs uvars vars (sheapD s)) stn sm
           /\ ST.HT.satisfies sm m) ->
-        match exprD_ptr_w funcs uvars vars pe , exprD_word funcs uvars vars ve with
-          | Some p , Some v =>
+        match exprD_ptr_w funcs uvars vars pe with
+          | Some p =>
             exists sm, 
                  ST.satisfies cs (sexprD funcs sfuncs uvars vars (sheapD s')) stn sm
               /\ ST.HT.satisfies sm (ST.HT.mem_set_word (IL.explode stn) p v m)
-          | _ , _ => False
+          | _ => False
         end.
       Proof.
         unfold symeval_write_word. intros.
@@ -555,587 +712,59 @@ Module Evaluator (B : Heap) (ST : SepTheoryX.SepTheoryXType B).
             case_eq (fold_known_update A B C D E); intros; try congruence
         end.
         eapply fold_known_update_correct in H.
-        do 5 destruct H. destruct H1.
-        intuition. inversion H2; clear H2; subst. 
+        do 5 destruct H. destruct H2.
+        intuition. inversion H3; clear H3; subst. 
         
-        eapply fold_args_update_correct in H5.
+        eapply fold_args_update_correct in H6.
         repeat match goal with
                  | [ H : exists x, _ |- _ ] => destruct H
                end. intuition; subst.
-        generalize (sheapD_pures _ _ _ _ _ H3).
-        rewrite sheapD_pull_impure in H3 by eauto.
-        assert (In x7 (x5 ++ x7 :: x6)). 
-        apply in_or_app; right; simpl; auto.
-        eapply starred_In in H5.
-        destruct H5. rewrite H5 in H3.
-        rewrite <- heq_star_assoc in H3. rewrite heq_star_comm in H3.
+        generalize (sheapD_pures _ _ _ _ _ H4).
+        rewrite sheapD_pull_impure in H4 by eauto.
+        rewrite starred_In in H4.
+        rewrite <- heq_star_assoc in H4. rewrite heq_star_comm in H4.
         
-        simpl in *. rewrite H1 in *.
+        simpl in *. rewrite H2 in *.
         intros.
-        eapply sym_write_word_correct in H2; eauto.
+
+        eapply sym_write_word_correct 
+          with (P := ST.star
+            (sexprD funcs sfuncs uvars vars0
+              (sheapD
+                {|
+                  impures := FM.remove x (impures s);
+                  pures := pures s;
+                  other := other s |}))
+            (sexprD funcs sfuncs uvars vars0 (starred (Func x) (x5 ++ x6) Emp)))
+            (stn := stn) (cs := cs) (m := x4)
+          in H3; eauto.
         2: apply AllProvable_app; eauto.
-
-        Focus 2.
-
-        generalize dependent H3.
+        destruct (exprD_ptr_w funcs uvars vars0 pe); eauto.
+        unfold tvarD in H3.
+        exists (ST.HT.smem_set_word (IL.explode stn) a v x4). split.
+        2: eapply ST.HT.satisfies_set_word; eauto.
+        rewrite sheapD_pull_impure.
+        2: eapply FM.find_add.
+        rewrite starred_In.
+        simpl. rewrite H2. generalize dependent H3. 
         match goal with
           | [ |- context [ applyD ?A ?B ?C ?D ?E ] ] =>
             case_eq (applyD A B C D E)
         end. intros.
-        generalize (sym_write_word_correct).
-        
+        rewrite <- ST.heq_star_assoc. rewrite ST.heq_star_comm. 
+        rewrite FM.remove_add. eapply H7.
+        intros; exfalso; auto.
 
-      Admitted.
+        unfold tvarD. generalize dependent H4.
+        match goal with
+          | [ |- context [ applyD ?A ?B ?C ?D ?E ] ] =>
+            case_eq (applyD A B C D E)
+        end. intros. auto.
+        intros. eapply ST.satisfies_star in H7.
+        do 2 destruct H7. intuition.
+        apply ST.satisfies_pure in H8. PropXTac.propxFo.
+      Qed.
 
     End WordAccess.
-
-(*
-
-    (** The full tactic **)
-    (** TODO : I really want to abstract this so that I don't have to rewrite it for
-     ** each read and write size
-     **)
-
-    Variable sfuncs : list (ssignature types (tvType pcIndex) (tvType stateIndex)).
-
-    Variable known : list nat. 
-    Variable evals : hlist (fun n : nat => match nth_error sfuncs n with
-                                             | None => Empty_set 
-                                             | Some ss => SymEval_byte ss
-                                           end) known.
-
-    Definition symeval_read_byte (hyps : list (expr types)) (p : expr types) 
-      (s : SHeap types (tvType pcIndex) (tvType stateIndex))
-      : option (expr types) :=
-      let hyps := hyps ++ pures s in
-      let reader _ seb args := 
-        sym_read_byte seb hyps args p
-      in
-      fold_known reader (impures s) evals.
-
-    Theorem symeval_read_byte_correct : forall cs stn hyps funcs pe ve s uvars vars (m : B.mem),
-      symeval_read_byte hyps pe s = Some ve ->
-      AllProvable funcs uvars vars hyps ->
-      (exists sm, 
-           ST.satisfies cs (sexprD funcs sfuncs (sheapD s) uvars vars) stn sm
-        /\ ST.HT.satisfies sm m) ->
-      match exprD_ptr funcs uvars vars pe , exprD_byte funcs uvars vars ve with
-        | Some p , Some v => 
-          B.mem_get m p = Some v
-        | _ , _ => False
-      end.
-    Proof.
-      unfold symeval_read_byte. intros.
-      eapply fold_known_correct in H.
-      do 5 destruct H. destruct H1.
-      intuition.
-
-      generalize (sheapD_pures _ _ _ _ _ H); intros.
-
-      eapply sheapD_pull_impure 
-        with (funcs := funcs) (sfuncs := sfuncs) (a := uvars) (c := vars0) (cs := cs)
-        in H1.
-      eapply starred_In in H3.
-      destruct H3. rewrite H3 in H1.
-
-      eapply sym_read_byte_correct 
-        with (funcs := funcs) (uvars := uvars) (vars := vars0) (cs := cs) (stn := stn) (m := x4)
-        in H6.
-      3: instantiate (1 := sexprD funcs sfuncs (Star
-            (sheapD
-               {|
-               impures := FM.remove x (impures s);
-               pures := pures s;
-               other := other s |})
-            (starred (Func x) x5 Emp)) uvars vars0).
-      destruct (exprD_ptr funcs uvars vars0 pe); auto.
-      destruct (exprD_byte funcs uvars vars0 ve); auto.
-      erewrite ST.HT.satisfies_get; eauto.
-
-      eapply AllProvable_app; auto.
-
-      unfold heq in *.
-      rewrite H1 in H. simpl in *. rewrite ST.heq_star_comm in H.
-      rewrite H2 in *. rewrite ST.heq_star_assoc in H.
-      rewrite ST.heq_star_comm in H. rewrite ST.heq_star_assoc in H.
-      generalize H. clear.
-      match goal with 
-        | [ |- context [ applyD ?A ?B ?C ?D ?E ] ] =>
-          destruct (applyD A B C D E)
-      end; auto.
-      clear. intros.
-      eapply ST.satisfies_star in H. do 2 destruct H. intuition.
-      eapply ST.satisfies_pure in H0. PropXTac.propxFo.
-    Qed.
-
-    Definition symeval_write_byte (hyps : list (expr types)) (p v : expr types) 
-      (s : SHeap types (tvType pcIndex) (tvType stateIndex))
-      : option (SHeap types (tvType pcIndex) (tvType stateIndex)) :=
-      let hyps := hyps ++ pures s in
-      let writer _ seb args := 
-        sym_write_byte seb hyps args p v
-      in
-      match fold_known_update writer (impures s) evals with
-        | None => None
-        | Some i' => Some {| impures := i' ; pures := pures s ; other := other s |}
-      end.
-
-    Theorem symeval_write_byte_correct : forall cs stn hyps funcs pe ve s s' uvars vars (m : B.mem),
-      symeval_write_byte hyps pe ve s = Some s' ->
-      AllProvable funcs uvars vars hyps ->
-      (exists sm, 
-           ST.satisfies cs (sexprD funcs sfuncs (sheapD s) uvars vars) stn sm
-        /\ ST.HT.satisfies sm m) ->
-      match exprD_ptr funcs uvars vars pe , exprD_byte funcs uvars vars ve with
-        | Some p , Some v =>
-          exists sm, 
-             ST.satisfies cs (sexprD funcs sfuncs (sheapD s') uvars vars) stn sm
-          /\ ST.HT.satisfies sm (B.mem_set m p v)
-        | _ , _ => False
-      end.
-    Proof.
-    Admitted.
-*)
   End typed.
 End Evaluator.
-
-
-(*
-    Lemma wordType_get : tvarD types (tvType wordIndex) = W.
-      unfold types. 
-    Admitted.
-
-    Definition exprD_word (funcs : functions types) (uvars vars : env types) (e : expr types) : 
-      option W :=
-      match wordType_get in _ = t return option t with
-        | refl_equal =>
-          @exprD types funcs uvars vars e (tvType wordIndex)
-      end.
-
-
-
-
-    Record SymEval (Predicate : ssignature types (tvType pcIndex) (tvType stateIndex)) : Type :=
-    { sym_read_word  : 
-      forall (hyps args : list (expr types)) (p : expr types), option (expr types)
-    ; sym_write_word : 
-      forall (hyps args : list (expr types)) (p v : expr types),
-        option (list (expr types))
-    ; sym_read_word_correct : forall funcs args uvars vars cs hyps pe ve m s,
-      sym_read_word hyps args pe = Some ve ->
-      AllProvable funcs nil nil  hyps ->
-      match 
-        applyD (@exprD _ funcs uvars vars) (SDomain Predicate) args _ (SDenotation Predicate)
-        with
-        | None => False
-        | Some p => ST.satisfies cs p s m
-      end ->
-      match exprD_ptr uvars vars pe , exprD_word uvars vars ve with
-        | Some p , Some v =>
-          smem_get p m = Some v
-        | _ , _ => False
-      end
-(*
-    ; sym_write_correct : forall funcs args uvars vars P cs hyps pe ve v m s args',
-      sym_write hyps args pe ve = Some args' ->
-      hlist (FalseDefault funcs) hyps ->
-      exprD funcs uvars vars ve pcType = Some v ->
-      match applyD (@exprD types funcs uvars vars) (SDomain Predicate) args _ (SDenotation Predicate) with
-        | None => False
-        | Some p => ST.satisfies (ST.star p P) cs s m
-      end ->
-      match exprD funcs uvars vars pe pcType with
-        | Some p =>
-          match applyD (@exprD types funcs uvars vars) (SDomain Predicate) args' _ (SDenotation Predicate) with
-            | None => False
-            | Some pr => ST.satisfies (ST.star pr P) cs s (WriteWord s m p v)
-          end
-        | _ => False
-      end
-*)
-    }.
-
-    Definition defaultSymEval (P : ssignature types pcType stateType) : SymEval.
-    refine (
-      {| Predicate             := P
-       ; sym_read_word         := fun _ _ _ => None
-       ; sym_write_word        := fun _ _ _ _ => None
-       ; sym_read_word_correct := _
-(*       ; sym_write_correct := _ *)
-       |}); 
-    abstract (simpl; intros; congruence).
-    Defined.
-
-    Section evaluator.
-      Fixpoint matches (sfuncs : list (ssignature types pcType stateType)) (evals : list (option SymEval)) : Prop :=
-        match evals with
-          | nil => True
-          | e :: es =>
-            match sfuncs with
-              | nil => False
-              | s :: ss =>
-                match e with
-                  | None => True
-                  | Some e => Predicate e = s 
-                end /\ matches ss es
-            end
-        end.
-
-      Variable evals : list (option SymEval).
-
-      Section fold_find.
-        Variable T U : Type.
-        Variable F : nat -> T -> option U.
-        
-        Fixpoint fold_find (m : FM.t T) : option (nat * U) :=
-          match m with 
-            | FM.MLeaf => None
-            | FM.MBranch l k v r =>
-              match F k v with
-                | Some z => Some (k, z)
-                | None => 
-                  match fold_find l with
-                    | None => fold_find r 
-                    | Some k => Some k
-                  end
-              end
-          end.
-
-        Variable D : nat -> T -> sexpr types pcType stateType.
-        Variable P : nat -> T -> tvarD types stateType -> Prop.
-        Variable funcs : functions types.
-        Variable sfuncs : list (ssignature types pcType stateType).
-
-        Hypothesis imp : forall cs uv vs k v m,
-             ST.satisfies (sexprD funcs sfuncs (D k v) uv vs) cs (fst m) (Mem (snd m)) 
-          -> P k v m.
-        Hypothesis ext : forall cs uv vs k v m,
-             ST.satisfies (sexprD funcs sfuncs (D k v) uv vs) cs (fst m) (Mem (snd m)) 
-          -> forall p m',
-               ST.satisfies (ST.star (sexprD funcs sfuncs (D k v) uv vs) p) cs (fst m') (Mem (snd m'))
-               -> P k v m'.
-        Hypothesis FD : forall k v u m,
-          F k v = Some u -> P k v m.
-
-(*
-        Theorem fold_find_ind : forall m, 
-          fold_find 
-*)
-      End fold_find.
-
-      
-
-
-      Definition symeval_read (hyps : list (expr types)) (p : expr types) (s : SHeap types pcType stateType) 
-        : option (expr types) :=
-        let hyps := hyps ++ pures s in
-        let res := 
-          fold_find (fun k v => 
-            match nth_error evals k with
-              | Some (Some ev) =>
-                let reader := sym_read ev hyps in
-                  List.fold_left (fun acc args =>
-                    match acc with
-                      | Some _ => acc
-                      | None => reader args p 
-                    end) v None
-              | _ => None
-            end)
-          (impures s)
-        in match res with
-             | None => None
-             | Some a => Some (snd a)
-           end.
-
-      Variable funcs : functions types.
-      Variable sfuncs : list (ssignature types pcType stateType).
-      Hypothesis evals_matches : matches sfuncs evals.
-
-      Definition symeval_read_correct : forall hyps pe s ve,
-        symeval_read hyps pe s = Some ve ->
-        hlist (FalseDefault funcs) hyps ->
-        forall uvars vars cs stn m,
-        ST.satisfies (@sexprD types funcs pcType stateType sfuncs (SEP.sheapD s) uvars vars) cs stn m -> 
-        match exprD funcs uvars vars ve pcType , exprD funcs uvars vars pe pcType with
-          | Some v , Some p => ReadWord stn m p = v 
-          | _ , _ => False
-        end.
-      Proof.
-        Opaque tvarD.
-        unfold symeval_read. destruct s; simpl.
-        induction impures0; simpl in *.
-          intros; congruence.
-
-          intros.
-          cut (ST.satisfies (sexprD funcs sfuncs (sheapD {| impures := impures0_1 ; pures := pures0 ; other := other0 |}) uvars vars0) cs stn m).
-          cut (ST.satisfies (sexprD funcs sfuncs (sheapD {| impures := impures0_2 ; pures := pures0 ; other := other0 |}) uvars vars0) cs stn m).
-          Focus.
-
-          Ltac head x :=
-            match x with
-              | match ?y with
-                  | Some _ => _
-                  | None => _
-                end => head y
-              | _ => x
-            end.
-
-          Print ST.
-          Ltac more :=
-          repeat match goal with
-                   | [  H' : _ |- _ ] => 
-                     specialize (H' _ (refl_equal _))
-                   | [ H : hlist (FalseDefault _) _, H' : _  |- _ ] =>
-                     specialize (H' H)
-                   | [ H : ST.satisfies _ _ _ _ , H' : _  |- _ ] =>
-                     specialize (H' _ _ _ _ _ H)
-                   | _ => solve [ eauto ] 
-                   | [ H : Some _ = Some _ |- _ ] => inversion H; clear H; try subst
-                   | [ H : forall x, None = Some x -> _ |- _ ] => clear H
-                   | [ H : context [ match ?X with
-                                       | Some _ => _
-                                       | None => _
-                                     end ] |- _ ] =>
-                   let X := head X in
-                     match X with 
-                       | fold_left _ _ _ =>
-                         generalize dependent H; case_eq (X); intros
-                       | fold_find _ _ =>
-                         generalize dependent X; let H := fresh in intro H; destruct H; intros
-(*
-                          (idtac "matched fold_find";
-                          intros; generalize dependent H; case_eq X;
-                            [ idtac "a"; let z := fresh "p" in intro z; let H' := fresh in intro H'; idtac "trying to rw"; 
-                              let v := eval unfold H' in H' in idtac v ; rewrite H' in *; idtac "a done" |
-                              idtac "b"; let H' := fresh in intros H'; rewrite H' in * ; idtac "b done" ]; intros ; idtac "completed")
-*)
-
-                       | exprD _ _ _ _ _ => fail 2
-                     end
-                   | _ => congruence
-                 end; eauto.
-          destruct (nth_error evals n); intros; more; try destruct o; more.
-          Print sheapD.
-          Lemma scan_function_correct : forall uvars vars0 t cs stn m pe ve k hyps s acc,
-            fold_left
-            (fun (acc : option (expr types)) (args : list (expr types)) =>
-              match acc with
-                | Some _ => acc
-                | None => sym_read s hyps args pe
-              end) t acc = Some ve ->
-            match acc with
-              | None => True
-              | Some ve =>
-                match exprD funcs uvars vars0 ve pcType with
-                  | Some v =>
-                    match exprD funcs uvars vars0 pe pcType with
-                      | Some p0 => ReadWord stn m p0 = v
-                      | None => False
-                    end
-                  | None => False
-                end
-            end ->                
-            nth_error evals k = Some (Some s) ->
-            ST.satisfies (@sexprD types funcs pcType stateType sfuncs (starred' (Func k) t Emp) uvars vars0) cs stn m ->
-            match exprD funcs uvars vars0 ve pcType with
-              | Some v =>
-                match exprD funcs uvars vars0 pe pcType with
-                  | Some p0 => ReadWord stn m p0 = v
-                  | None => False
-                end
-              | None => False
-            end.
-          Proof.
-            induction t; simpl in *.
-              intros; subst; auto.
-
-              intros. destruct acc.
-              assert (e = ve).
-              generalize H. clear.
-              induction t; eauto; simpl; congruence.
-              subst. eauto.
-              eapply IHt; eauto.
-              assert (nth_error sfuncs k = Some (Predicate s)).
-              Focus.
-              generalize H1. generalize evals_matches. clear. generalize sfuncs. clear. induction evals; simpl.
-                destruct k; intros; simpl in *. inversion H1. inversion H1.
-                destruct sfuncs; simpl in *; intros; try intuition.
-                destruct k; simpl in *. inversion H1; clear H1; subst. subst. reflexivity.
-                eapply IHl in H0; eauto.
-                
-
-                destruct k. simpl. inversion 2. subst. destruct sfuncs; auto.
-                simpl in *; eauto. intuition. subst. reflexivity.
-                destruct sfuncs; intuition. 
-
-              simpl in *. dest
-              
-  (*
-End Evaluator.
-*)
-
-
-
-  Section ptsto32_sym_eval.
-    Definition denotesTo (sfuncs : list (ssignature types pcType stateType)) (f : nat) 
-      (Predicate : ssignature types pcType stateType) : Prop :=
-      nth_error sfuncs f = Some Predicate.
-
-    Record SymEval : Type :=
-      { Predicate : ssignature types pcType stateType
-      ; sym_read  : 
-        forall (hyps args : list (expr types)) (p : expr types), option (expr types)
-      ; sym_write : 
-        forall (hyps : list (expr types)) (f : nat) (args : list (expr types)) (p v : expr types),
-          option (sexpr types pcType stateType)
-      ; sym_read_correct : forall funcs sfuncs f args uvars vars P cs
-          hyps
-          pe ve m s,
-        denotesTo sfuncs f Predicate ->
-        sym_read hyps args pe = Some ve ->
-        hlist (FalseDefault funcs) hyps ->
-        ST.satisfies 
-          (@sexprD types funcs pcType stateType sfuncs (Star (Func f args) P) uvars vars)
-          cs s m ->
-        match exprD funcs uvars vars pe pcType , exprD funcs uvars vars ve pcType with
-          | Some p , Some v =>
-            ReadWord s m p = v 
-          | _ , _ => False
-        end
-      ; sym_write_correct : forall funcs sfuncs f args uvars vars P cs
-          hyps
-          (pfW : tvarD types pcType = W)
-          pe ve v m s s',
-        denotesTo sfuncs f Predicate ->
-        sym_write hyps f args pe ve = Some s' ->
-        hlist (FalseDefault funcs) hyps ->
-        exprD funcs uvars vars ve pcType = Some v ->
-        ST.satisfies 
-          (@sexprD types funcs pcType stateType sfuncs (Star (Func f args) P) uvars vars)
-          cs s m ->
-        match exprD funcs uvars vars pe pcType with
-          | Some p =>
-            ST.satisfies 
-              (@sexprD types funcs pcType stateType sfuncs (Star s' P) uvars vars)
-              cs s (WriteWord s m p v)
-          | _ => False
-        end
-      }.
-
-
-    Definition btypes : list type := bedrock_types.
-    Variable types : list type.
-
-    Definition ptsto32_Predicate : ssignature (btypes ++ types) pcType stateType :=
-      Build_ssignature (btypes ++ types) pcType stateType (pcType :: pcType :: nil) (@ptsto32 nil).
-      
-  (** Let's see how this works with ptsto **)
-    Definition ptsto32_sym_read (hyps args : list (expr (btypes ++ types))) (p : expr (btypes ++ types)) : option (expr (btypes ++ types)) :=
-      match args with
-        | p' :: v :: nil =>
-          if seq_dec p p' then Some v else None
-        | _ => None
-      end.
-
-    Definition ptsto32_sym_write (hyps : list (expr (btypes ++ types))) f (args : list (expr (btypes ++ types))) (p v : expr (btypes ++ types)) : option (sexpr (btypes ++ types) pcType stateType) :=
-      match args with
-        | p' :: v :: nil =>
-          if seq_dec p p' then Some (Func f (p' :: v :: nil)) else None
-        | _ => None
-      end.
-
-    Require Import PropXTac.
-
-    Theorem ptsto32_sym_read_correct : forall (funcs : functions (Top.types types))
-     (sfuncs : list (ssignature (Top.types types) pcType stateType))
-     (f : nat) (args : list (expr (Top.types types)))
-     (uvars vars0 : list {t : tvar & tvarD (Top.types types) t})
-     (P : sexpr (Top.types types) pcType stateType)
-     (cs : PropX.codeSpec (tvarD (Top.types types) pcType)
-             (tvarD (Top.types types) stateType))
-     (hyps : list (expr (Top.types types))) (pe ve : expr (Top.types types))
-     (m : BedrockHeap.mem) (s : settings),
-     denotesTo sfuncs f ptsto32_Predicate ->
-     ptsto32_sym_read hyps args pe = Some ve ->
-     hlist (FalseDefault funcs) hyps ->
-     ST.satisfies (sexprD funcs sfuncs (Star (Func f args) P) uvars vars0) cs s
-     m ->
-     match exprD funcs uvars vars0 pe pcType , exprD funcs uvars vars0 ve pcType with
-       | Some p , Some v => ReadWord s m p = v
-       | _ , _ => False
-     end.
-    Proof.
-      intros.
-      destruct args; simpl in H0; try congruence.
-      destruct args; simpl in H0; try congruence.
-      destruct args; simpl in H0; try congruence.
-      unfold denotesTo in *. simpl in *. rewrite H in H1; clear H. simpl in *. 
-      repeat match goal with
-        | [ H : (if ?X then Some _ else None) = Some _ |- _ ] =>
-          destruct X; inversion H; clear H; subst
-        | [ |- match ?X with
-                 | Some _ => _
-                 | None => False
-               end ] => destruct X
-      end;
-      destruct H1 as [ ? [ ? ? ] ]; try solve [ propxFo ].
-      propxFo. unfold implode in H8. subst.
-      eapply satisfies_split in H1; eauto. destruct H1.
-      repeat match goal with 
-               | [ H : smem_get _ _ = _ |- _ ] =>
-                 eapply satisfies_get in H; [ | eassumption ]; unfold BedrockHeap.mem_get in H; inversion H; subst
-             end;
-      eapply ReadWordFootprint; simpl; auto.
-    Qed.
-
-    Theorem ptsto32_sym_write_correct : forall (funcs : functions (Top.types types))
-      (sfuncs : list (ssignature (Top.types types) pcType stateType))
-      (f : nat) (args : list (expr (Top.types types)))
-      (uvars vars0 : env (Top.types types))
-      (P : sexpr (Top.types types) pcType stateType)
-      (cs : PropX.codeSpec (tvarD (Top.types types) pcType)
-        (tvarD (Top.types types) stateType))
-      (hyps : list (expr (Top.types types))),
-      tvarD (Top.types types) pcType = W ->
-      forall (pe ve : expr (Top.types types))
-        (v : tvarD (Top.types types) pcType) (m : BedrockHeap.mem)
-        (s : settings) (s' : sexpr (Top.types types) pcType stateType),
-        denotesTo sfuncs f ptsto32_Predicate ->
-        ptsto32_sym_write hyps f args pe ve = Some s' ->
-        hlist (FalseDefault funcs) hyps ->
-        exprD funcs uvars vars0 ve pcType = Some v ->
-        ST.satisfies (sexprD funcs sfuncs (Star (Func f args) P) uvars vars0) cs s
-        m ->
-        match exprD funcs uvars vars0 pe pcType with
-          | Some p =>
-            ST.satisfies (sexprD funcs sfuncs (Star s' P) uvars vars0) cs s
-            (WriteWord s m p v)
-          | None => False
-        end.
-    Proof.
-      intros.
-      destruct args; simpl in H1; try congruence.
-      destruct args; simpl in H1; try congruence.
-      destruct args; simpl in H1; try congruence.
-      unfold denotesTo in *. simpl in *. rewrite H0 in H3; clear H0. simpl in *. 
-      repeat match goal with
-               | [ H : (if ?X then Some _ else None) = Some _ |- _ ] =>
-                 destruct X; inversion H; clear H; subst
-               | [ |- match ?X with
-                        | Some _ => _
-                        | None => False
-                      end ] => destruct X
-             end;
-      destruct (exprD funcs uvars vars0 e0 pcType); destruct H3 as [ ? [ ? ? ] ]; propxFo.
-    Admitted.
-
-    Definition SymEval_ptsto32 : SymEval types :=
-      {| Predicate := ptsto32_Predicate
-       ; sym_read  := ptsto32_sym_read
-       ; sym_write := ptsto32_sym_write
-       ; sym_read_correct := ptsto32_sym_read_correct
-       ; sym_write_correct := ptsto32_sym_write_correct
-      |}.
-
-  End  ptsto32_sym_eval.
-*)
